src/Lustre/Normalization/NTyping.v
@@ -3,7 +3,7 @@ From Velus Require Import Common Ident.
 From Velus Require Import Operators Environment.
 From Velus Require Import CoindStreams.
 From Coq Require Import List. Import List.ListNotations. Open Scope list_scope.
-From Velus Require Import Lustre.LSyntax Lustre.LTyping Lustre.LClocking.
+From Velus Require Import Lustre.LSyntax Lustre.LTyping.
 From Velus Require Import Lustre.Normalization.Fresh Lustre.Normalization.FullNorm.
 
 (** * Preservation of Typing through Normalization *)
